CommunicationClosure.lean
@@ -3,6 +3,8 @@
 import CommunicationClosure.Protocols.Paxos
 import CommunicationClosure.Protocols.Raft
 import CommunicationClosure.Protocols.RaftWithHistory
+import CommunicationClosure.Protocols.RaftWithHistoryAndNetwork
 import CommunicationClosure.Proofs.Paxos
 import CommunicationClosure.Proofs.Raft
 import CommunicationClosure.Proofs.RaftWithHistory
+import CommunicationClosure.Proofs.RaftWithHistoryAndNetwork
